Proved `tokens_to_bytes_correctness`, but `compress'_valid_tokens` needs new proof.

lz78/LZ_Tokens.v
@@ -8,11 +8,13 @@ Module Tokens.
     | Tok (index: nat) (next: byte)
     | Last (index: nat).
 
-  Fixpoint valid_tokens (tokens: list Token) :=
+  Fixpoint valid_tokens (tokens: list Token) (dict_size: nat) :=
     match tokens with
-    | Tok _ _ :: rest => valid_tokens rest
+    | Tok index _ :: rest => index < 256 ^ (num_bytes_for_dict dict_size)
+                               /\ valid_tokens rest (S dict_size)
     | Last _ :: _ :: _ => False
-    | _ => True
+    | [Last index] => index < 256 ^ (num_bytes_for_dict dict_size) 
+    | [] => True
     end.
 
   Definition nat_to_byte (n: nat): byte :=
@@ -107,17 +109,141 @@ Module Tokens.
         lia.
   Qed.
 
-  (* The Hypothesis are not strong enough! *)
+  Lemma nat_to_k_bytes_length: forall k n,
+    length (nat_to_k_bytes k n) = k.
+  Proof.
+    induction k; simpl; intros.
+    - reflexivity.
+    - now rewrite IHk.
+  Qed.
+
+  Lemma app_l_eq_length {A}: forall n, forall l1 l2 l3 l4: list A,
+    l1 ++ l2 = l3 ++ l4 ->
+    length l1 = n -> length l3 = n ->
+    l1 = l3.
+  Proof.
+    induction n; intros.
+    - apply length_zero_iff_nil in H0, H1.
+      congruence.
+    - destruct l1, l3; simpl in *; try lia.
+      inversion H. subst.
+      specialize (IHn l1 l2 l3 l4 H4 ltac:(lia) ltac:(lia)).
+      congruence.
+  Qed.
+
   Lemma tokens_to_bytes_correctness': forall fuel tokens dict_size bytes,
     length bytes <= fuel ->
-    valid_tokens tokens ->
+    valid_tokens tokens dict_size ->
     tokens_to_bytes' dict_size tokens = bytes ->
     bytes_to_tokens' fuel dict_size bytes = tokens.
   Proof.
-  Admitted.
+    induction fuel; simpl; intros.
+    - destruct tokens. reflexivity.
+      inversion H.
+      apply length_zero_iff_nil in H3.
+      subst.
+      destruct t; simpl in H3.
+      + apply app_eq_nil in H3.
+        destruct H3.
+        discriminate.
+      + pose proof (num_bytes_for_dict_gt_one dict_size).
+        destruct (num_bytes_for_dict dict_size).
+        * lia.
+        * simpl in H3.
+          discriminate.
+    - destruct bytes.
+      + destruct tokens. reflexivity.
+        destruct t; simpl in H1.
+        * apply app_eq_nil in H1.
+          destruct H1.
+          discriminate.
+        * pose proof (num_bytes_for_dict_gt_one dict_size).
+          destruct (num_bytes_for_dict dict_size).
+          -- lia.
+          -- simpl in H1.
+             discriminate.
+      + destruct (length (b :: bytes) <? num_bytes_for_dict dict_size) eqn:?.
+        * destruct tokens. reflexivity.
+          simpl in H1.
+          apply Nat.ltb_lt in Heqb0.
+          destruct t.
+          -- pose proof (nat_to_k_bytes_length (num_bytes_for_dict dict_size) index).
+             assert (length (nat_to_k_bytes (num_bytes_for_dict dict_size) index)
+                      <= length (b :: bytes)). {
+               rewrite <- H1, length_app.
+               lia.
+             }
+             lia.
+          -- pose proof (nat_to_k_bytes_length (num_bytes_for_dict dict_size) index).
+             rewrite H1 in H2.
+             lia.
+        * destruct (length (b :: bytes) =? num_bytes_for_dict dict_size) eqn:?.
+          -- destruct tokens; simpl in H1.
+             ++ discriminate.
+             ++ destruct t.
+                ** apply Nat.eqb_eq in Heqb1.
+                   rewrite <- H1, length_app, nat_to_k_bytes_length in Heqb1.
+                   simpl in Heqb1. lia.
+                ** destruct tokens.
+                   --- rewrite <- H1, nat_to_k_bytes_correctness.
+                       +++ reflexivity.
+                       +++ now simpl in H0.
+                   --- simpl in H0. now exfalso.
+          -- destruct (skipn (num_bytes_for_dict dict_size) (b :: bytes)) eqn:?.
+             ++ apply Nat.ltb_ge in Heqb0.
+                apply Nat.eqb_neq in Heqb1.
+                apply skipn_all_iff in Heql.
+                lia.
+             ++ destruct tokens; simpl in H1.
+                ** discriminate.
+                ** destruct t.
+                   --- f_equal.
+                       +++ pose proof (firstn_skipn (num_bytes_for_dict dict_size) (b :: bytes)).
+                           rewrite Heql in H2.
+                           rewrite <- H2 in H1.
+                           assert (firstn (num_bytes_for_dict dict_size) (b :: bytes)
+                                   = nat_to_k_bytes (num_bytes_for_dict dict_size) index). {
+                             pose proof (nat_to_k_bytes_length (num_bytes_for_dict dict_size) index).
+                             eapply app_l_eq_length in H1.
+                             - congruence.
+                             - rewrite H3.
+                               reflexivity.
+                             - rewrite length_firstn.
+                               apply Nat.ltb_ge in Heqb0.
+                               apply Nat.eqb_neq in Heqb1.
+                               assert (Nat.min (num_bytes_for_dict dict_size) (length (b :: bytes))
+                                       = num_bytes_for_dict dict_size) by lia.
+                               now rewrite H4.
+                           }
+                           rewrite H3 in H1 |- *.
+                           rewrite nat_to_k_bytes_correctness.
+                           *** f_equal.
+                               apply app_inv_head in H1.
+                               congruence.
+                           *** simpl in H0.
+                               now destruct H0.
+                       +++ erewrite IHfuel.
+                           *** reflexivity.
+                           *** pose proof (length_skipn (num_bytes_for_dict dict_size) (b :: bytes)).
+                               rewrite Heql in H2.
+                               simpl in H2, H.
+                               destruct (num_bytes_for_dict dict_size); lia.
+                           *** simpl in H0.
+                               now destruct H0.
+                           *** rewrite <- H1 in Heql.
+                               pose proof (nat_to_k_bytes_length (num_bytes_for_dict dict_size) index).
+                               rewrite <- H2 in Heql at 1.
+                               rewrite skipn_app, Nat.sub_diag, skipn_all, skipn_0 in Heql.
+                               simpl in Heql.
+                               congruence.
+                   --- pose proof (nat_to_k_bytes_length (num_bytes_for_dict dict_size) index).
+                       rewrite H1 in H2.
+                       apply Nat.eqb_neq in Heqb1.
+                       lia.
+  Qed.
 
   Lemma tokens_to_bytes_correctness: forall tokens,
-    valid_tokens tokens ->
+    valid_tokens tokens 1 ->
     bytes_to_tokens (tokens_to_bytes tokens) = tokens.
   Proof.
     intros.
